nola/iris/plist.v
@@ -1,0 +1,25 @@
+(** * On [plist] *)
+
+From nola.util Require Export plist.
+From iris.bi Require Import bi.
+
+Fixpoint big_sepPL {PROP : bi} {A} {F : A → Type} (Φ : ∀ a, F a → PROP) {al}
+  : plist F al → PROP :=
+  match al with [] => λ _, emp | _ :: _ =>
+    λ '(x, xl)', Φ _ x ∗ big_sepPL Φ xl end%I.
+Notation "[∗ plist] a ; x ∈ xl , P" := (big_sepPL (λ a x, P) xl)
+  (at level 200, xl at level 10, a binder, x binder,
+    format "[∗  plist]  a ;  x  ∈  xl ,  P") : bi_scope.
+Notation "[∗ plist] x ∈ xl , P" := (big_sepPL (λ _ x, P) xl)
+  (at level 200, xl at level 10, x binder,
+    format "[∗  plist]  x  ∈  xl ,  P") : bi_scope.
+
+Section big_sepPL.
+  Context {PROP : bi} {A} {F : A → Type}.
+
+  (** [big_sepPL] over [of_plist] *)
+  Lemma big_sepPL_of_plist {B}
+    (f : ∀ a, F a → B) (Φ : B → PROP) {al} (xl : plist F al) :
+    ([∗ list] y ∈ of_plist f xl, Φ y) ⊣⊢ [∗ plist] x ∈ xl, Φ (f _ x).
+  Proof. move: xl. elim: al=>/=; [done|]=> ?? IH [??]. by rewrite IH. Qed.
+End big_sepPL.
