nola/util/plist.v
@@ -1,0 +1,59 @@
+(** * Product list *)
+
+From nola Require Export prod.
+From stdpp Require Import vector.
+
+(** Product list *)
+Fixpoint plist {A} (F : A → Type) (al : list A) : Type :=
+  match al with [] => unit | a :: al => F a *' plist F al end.
+
+(** [plist] as [list] *)
+Fixpoint of_plist {A} {F : A → Type} {B} (f : ∀ a, F a → B) {al}
+  : plist F al → list B :=
+  match al with [] => λ _, [] | _ :: _ =>
+    λ '(x, xl)', f _ x :: of_plist f xl end.
+
+(** Map [plist] *)
+Fixpoint plist_map {A} {F G : A → Type} (f : ∀ a, F a → G a) {al : list A}
+  : plist F al → plist G al :=
+  match al with [] => λ _, () | _ :: _ =>
+    λ '(x, xl)', (f _ x, plist_map f xl)' end.
+
+(** Zip [plist]s *)
+Fixpoint plist_zip {A} {F G : A → Type} {al : list A}
+  : plist F al → plist G al → plist (λ a, F a *' G a) al :=
+  match al with [] => λ _ _, () | _ :: _ =>
+    λ '(x, xl)' '(y, yl)', ((x, y)', plist_zip xl yl)' end.
+
+(** [plist] over [repeat] as [vec] *)
+Fixpoint of_plist_repeat {A} {F : A → Type} {a : A} {n}
+  : plist F (repeat a n) → vec (F a) n :=
+  match n with 0 => λ _, [#] | S _ =>
+    λ '(x, xl)', x ::: of_plist_repeat xl end.
+Fixpoint to_plist_repeat {A} {F : A → Type} {a : A} {n} (xl : vec (F a) n)
+  : plist F (repeat a n) :=
+  match xl with [#] => () | b ::: xl => (b, to_plist_repeat xl)' end.
+Lemma to_of_plist_repeat {A F} {a : A} {n} {xl : plist F (repeat a n)} :
+  to_plist_repeat (of_plist_repeat xl) = xl.
+Proof. move: xl. elim: n=>/=; [by case|]=> ? IH [??]. by rewrite IH. Qed.
+Lemma of_to_plist_repeat {A F} {a : A} {n} {xl : vec (F a) n} :
+  of_plist_repeat (to_plist_repeat xl) = xl.
+Proof. by elim: xl=>/=; [done|]=> ???->. Qed.
+
+(** [plist] over [++] *)
+Fixpoint plist_app {A} {F : A → Type} {al bl}
+  : plist F al → plist F bl → plist F (al ++ bl) :=
+  match al with [] => λ _, id | _ :: _ =>
+    λ '(x, xl)' yl, (x, plist_app xl yl)' end.
+Fixpoint plist_sep {A} {F : A → Type} {al bl}
+  : plist F (al ++ bl) → plist F al *' plist F bl :=
+  match al with [] => λ xl, ((), xl)' | _ :: _ =>
+    λ '(x, xl)', let '(yl, zl)' := plist_sep xl in ((x, yl)', zl)' end.
+Lemma plist_app_sep {A} {F : A → Type} {al bl}
+  {xl : plist F al} {yl : plist F bl} :
+  plist_sep (plist_app xl yl) = (xl, yl)'.
+Proof. move: xl yl. elim: al=>/=; [by case|]=> ?? IH [??]?. by rewrite IH. Qed.
+Lemma plist_sep_app {A} {F : A → Type} {al bl}
+  {xl : plist F (al ++ bl)} :
+  plist_app (plist_sep xl).1' (plist_sep xl).2' = xl.
+Proof. move: xl. elim: al=>/=; [done|]=> ?? IH [??]. by rewrite IH. Qed.
